Prove splitting a step into promise; lower-only

src/sequential/Delayed.v
@@ -29,10 +29,13 @@ Require Import Pred.
 Require Import Trace.
 Require Import MemoryProps.
 Require Import LowerMemory.
+Require Import FulfillStep.
+Require Import ReorderStepPromise.
 
 Require Import gSimAux.
 
 Set Implicit Arguments.
+
 
 Definition is_promise (e: ThreadEvent.t): Prop :=
   match e with
@@ -54,19 +57,18 @@ Definition release_event (e: ThreadEvent.t): Prop :=
 
 Variant lower_step {lang} e (th0 th1: Thread.t lang): Prop :=
 | lower_step_intro
-    (STEP: Thread.step true e th0 th1)
-    (NPROMISE: no_promise e)
+    (STEP: Thread.program_step e th0 th1)
     (NRELEASE: ~ release_event e)
     (MEM: lower_memory th1.(Thread.memory) th0.(Thread.memory))
 .
 
-Lemma write_lower_memory_lower prom0 mem0 loc from to msg prom1 mem1 kind
-      (PROMISE: Memory.write prom0 mem0 loc from to msg prom1 mem1 kind)
-      (LOWER: lower_memory mem1 mem0)
-  :
-    exists msg, kind = Memory.op_kind_lower msg.
+Lemma write_lower_memory_lower
+      prom0 mem0 loc from to msg prom1 mem1 kind
+      (WRITE: Memory.write prom0 mem0 loc from to msg prom1 mem1 kind)
+      (LOWER: lower_memory mem1 mem0):
+  Memory.op_kind_is_lower kind.
 Proof.
-  inv PROMISE. inv PROMISE0; eauto.
+  inv WRITE. inv PROMISE; eauto.
   { eapply Memory.add_get0 in MEM. des.
     hexploit lower_memory_get_inv; eauto. i. des; clarify. }
   { eapply Memory.split_get0 in MEM. des.
@@ -75,19 +77,67 @@ Proof.
     hexploit lower_memory_get; eauto. i. des; clarify. }
 Qed.
 
-Lemma step_split_pure lang (th0 th2: Thread.t lang) e
-      (STEP: Thread.step true e th0 th2)
+Lemma write_na_future
+      ts prom0 mem0 loc from to msg prom1 mem1 msgs kinds kind
+      (WRITE: Memory.write_na ts prom0 mem0 loc from to msg prom1 mem1 msgs kinds kind):
+  Memory.future mem0 mem1.
+Proof.
+  induction WRITE.
+  - inv WRITE. exploit Memory.promise_op; eauto. i.
+    econs 2; eauto. econs; eauto.
+    econs. apply Time.bot_spec.
+  - etrans; try exact IHWRITE.
+    inv WRITE_EX. exploit Memory.promise_op; eauto. i.
+    econs 2; eauto. econs; eauto.
+    + unguard. des; subst; ss. econs. ss.
+    + unguard. des; subst; ss. econs. apply Time.bot_spec.
+Qed.
+
+Lemma write_na_lower_memory_lower
+      ts prom0 mem0 loc from to msg prom1 mem1 msgs kinds kind
+      (WRITE: Memory.write_na ts prom0 mem0 loc from to msg prom1 mem1 msgs kinds kind)
+      (LOWER: lower_memory mem1 mem0)
+  :
+    (<<KINDS: List.Forall (fun kind => Memory.op_kind_is_lower kind) kinds>>) /\
+    (<<KIND: Memory.op_kind_is_lower kind>>).
+Proof.
+  induction WRITE; eauto using write_lower_memory_lower.
+  exploit write_na_future; try exact WRITE. i.
+  inv WRITE_EX. inv PROMISE.
+  - exploit Memory.add_get0; try exact MEM. i. des.
+    exploit Memory.future_get1; try exact GET0; eauto.
+    { unguard. des; subst; ss. }
+    i. des.
+    inv LOWER. exploit LOWER0.
+    erewrite GET. erewrite GET1. i. inv x.
+  - exploit Memory.split_get0; try exact MEM. i. des.
+    exploit Memory.future_get1; try exact GET1; eauto. i. des.
+    inv LOWER. exploit LOWER0.
+    erewrite GET. erewrite GET3. i. inv x.
+  - cut (lower_memory mem2 mem').
+    { i. exploit IHWRITE; eauto. i. des. auto. }
+    econs. i.
+    erewrite (@Memory.lower_o mem'); eauto. condtac; ss.
+    + des. subst.
+      exploit Memory.lower_get0; try exact MEM. i. des.
+      exploit Memory.future_get1; try exact GET0; eauto. i. des.
+      inv LOWER. exploit LOWER0. erewrite GET. i. inv x.
+      rewrite <- H0 in *. inv GET1. econs. eauto.
+    + inv LOWER. eauto.
+  - unguard. des; subst; ss.
+Qed.
+
+Lemma step_split_pure
+      lang pf e (th1 th2: Thread.t lang)
+      (STEP: Thread.step pf e th1 th2)
       (NPROMISE: no_promise e)
       (NRELEASE: ~ release_event e)
-      (MEM: th2.(Thread.memory) = th0.(Thread.memory))
+      (MEM: th2.(Thread.memory) = th1.(Thread.memory))
   :
-    exists th1,
-      (<<PROMISES: rtc (tau (@pred_step is_promise _)) th0 th1>>) /\
-      (<<LOWER: rtc (tau lower_step) th1 th2>>) /\
-      (<<MEM: th1.(Thread.memory) = th2.(Thread.memory)>>) /\
-      (<<SC: th1.(Thread.sc) = th2.(Thread.sc)>>).
+    (<<LOWER: tau lower_step th1 th2>>) /\
+    (<<SC: th2.(Thread.sc) = th1.(Thread.sc)>>).
 Proof.
-  assert (SC: th2.(Thread.sc) = th0.(Thread.sc)).
+  assert (SC: th2.(Thread.sc) = th1.(Thread.sc)).
   { inv STEP; inv STEP0; auto. inv LOCAL; ss.
     { inv LOCAL0; ss. }
     { inv LOCAL1; inv LOCAL2; ss. }
@@ -98,14 +148,9 @@ Proof.
     }
     { inv LOCAL0; ss. }
   }
-  subst. esplits.
-  { econs. }
-  { econs; [|econs]. econs; eauto.
-    { econs; eauto. rewrite MEM. refl. }
-    { destruct e; ss. }
-  }
-  { auto. }
-  { auto. }
+  esplits; eauto. econs.
+  { inv STEP; [inv STEP0; ss|]. econs; eauto. rewrite MEM. refl. }
+  { destruct e; ss. }
 Qed.
 
 Lemma memory_op_diff_only
@@ -145,8 +190,8 @@ Proof.
     left. esplits; eauto. refl. }
 Qed.
 
-Lemma promise_step_tau_promise_step lang (th0 th1: Thread.t lang)
-      pf e
+Lemma promise_step_tau_promise_step
+      lang pf e (th0 th1: Thread.t lang)
       (STEP: Thread.promise_step pf e th0 th1)
   :
     tau (@pred_step is_promise _) th0 th1.
@@ -159,8 +204,8 @@ Proof.
   { inv STEP; ss. }
 Qed.
 
-Lemma lower_step_tau_lower_step lang (th0 th1: Thread.t lang)
-      e
+Lemma lower_step_tau_lower_step
+      lang e (th0 th1: Thread.t lang)
       (STEP: lower_step e th0 th1)
   :
     tau lower_step th0 th1.
@@ -193,21 +238,116 @@ Proof.
   econs; eauto.
 Qed.
 
-Lemma step_split lang (th0 th2: Thread.t lang) pf e
+Lemma split_memory_write
+      promises1 mem1 loc from to msg promises2 mem2 kind
+      (MESSAGE: msg <> Message.reserve)
+      (WRITE: Memory.write promises1 mem1 loc from to msg promises2 mem2 kind):
+  exists promises1',
+    (<<PROMISE: Memory.promise promises1 mem1 loc from to msg promises1' mem2 kind>>) /\
+    (<<WRITE_LOWER: Memory.write promises1' mem2 loc from to msg promises2 mem2 (Memory.op_kind_lower msg)>>).
+Proof.
+  exploit MemoryFacts.write_time_lt; eauto. i.
+  assert (MSG: Message.wf msg).
+  { inv WRITE. inv PROMISE; inv MEM; ss.
+    - inv ADD. ss.
+    - inv SPLIT. ss.
+    - inv LOWER. ss.
+  }
+  assert (MSG_TO: Memory.message_to msg loc to).
+  { inv WRITE. inv PROMISE; ss. }
+  inv WRITE. esplits; eauto.
+  exploit Memory.promise_get0; eauto.
+  { inv PROMISE; ss. }
+  i. des.
+  exploit Memory.lower_exists_same; try exact GET_PROMISES; eauto. i.
+  exploit Memory.lower_exists_same; try exact GET_MEM; eauto.
+Qed.
+
+Lemma split_write
+      lc0 sc0 mem0 loc from to val releasedm released ord lc2 sc2 mem2 kind
+      (REL_WF: View.opt_wf releasedm)
+      (REL_CLOSED: Memory.closed_opt_view releasedm mem0)
+      (WF0: Local.wf lc0 mem0)
+      (SC0: Memory.closed_timemap sc0 mem0)
+      (MEM0: Memory.closed mem0)
+      (ORD: Ordering.le ord Ordering.relaxed)
+      (STEP: Local.write_step lc0 sc0 mem0 loc from to val releasedm released ord lc2 sc2 mem2 kind):
+  exists released' lc1,
+    (<<RELEASED: released' = TView.write_released (Local.tview lc0) sc0 loc to releasedm ord>>) /\
+    (<<PROMISE: Local.promise_step lc0 mem0 loc from to
+                                   (Message.concrete val released') lc1 mem2 kind>>) /\
+    (<<WRITE: Local.write_step lc1 sc0 mem2 loc from to val releasedm released ord lc2 sc2 mem2
+                               (Memory.op_kind_lower (Message.concrete val released'))>>).
+Proof.
+  exploit write_promise_fulfill; eauto. i. des.
+  exploit Local.promise_step_future; eauto. i. des.
+  exploit fulfill_write; try exact STEP2; eauto.
+  subst. inv STEP1. ss.
+Qed.
+
+Lemma reorder_write_lower_rtc_promise
+      lang
+      promises1 mem1
+      loc from to msg kind
+      th2 th3
+      (LE: Memory.le promises1 mem1)
+      (KIND: Memory.op_kind_is_lower kind)
+      (WRITE: Memory.write promises1 mem1 loc from to msg
+                           th2.(Thread.local).(Local.promises) th2.(Thread.memory) kind)
+      (STEPS: rtc (tau (@pred_step is_promise lang)) th2 th3):
+  exists th2',
+    (<<STEPS: rtc (tau (@pred_step is_promise lang))
+                  (Thread.mk _ th2.(Thread.state)
+                             (Local.mk th2.(Thread.local).(Local.tview) promises1)
+                             th2.(Thread.sc) mem1)
+                  th2'>>) /\
+    (<<WRITE: Memory.write th2'.(Thread.local).(Local.promises) th2'.(Thread.memory)
+                           loc from to msg
+                           th3.(Thread.local).(Local.promises) th3.(Thread.memory) kind>>) /\
+    (<<STATE: th2'.(Thread.state) = th3.(Thread.state)>>) /\
+    (<<TVIEW: th2'.(Thread.local).(Local.tview) = th3.(Thread.local).(Local.tview)>>) /\
+    (<<SC: th2'.(Thread.sc) = th3.(Thread.sc)>>).
+Proof.
+  revert promises1 mem1 LE WRITE.
+  induction STEPS; i.
+  { esplits; try refl. ss. }
+  inv H. inv TSTEP. inv STEP. inv STEP0; inv STEP; inv LOCAL; ss.
+  exploit reorder_memory_write_lower_promise; try exact WRITE; eauto. i. des.
+  hexploit Memory.promise_le; try exact PROMISE0; eauto. i. des.
+  exploit IHSTEPS; eauto. i. des.
+  esplits; try exact WRITE1; eauto.
+  econs 2; eauto. econs.
+  - econs; [do 4 econs; eauto|]; ss.
+    inv WRITE0. inv PROMISE1; ss.
+    eapply lower_closed_message_inv; eauto.
+  - ss.
+Qed.
+
+Lemma memory_write_lower_refl_inv
+      promsies1 mem1 loc from to msg promises2 mem2
+      (WRITE: Memory.write promsies1 mem1 loc from to msg promises2 mem2 (Memory.op_kind_lower msg)):
+  mem1 = mem2.
+Proof.
+  inv WRITE. inv PROMISE; ss.
+  apply Memory.ext. i.
+  exploit Memory.lower_get0; try exact MEM. i. des.
+  erewrite (@Memory.lower_o mem2); eauto. condtac; ss.
+  des. subst. ss.
+Qed.
+
+Lemma split_step
+      lang pf e (th0 th2: Thread.t lang)
       (STEP: Thread.step pf e th0 th2)
       (NRELEASE: ~ release_event e)
       (LOCAL: Local.wf (Thread.local th0) (Thread.memory th0))
       (SC: Memory.closed_timemap (Thread.sc th0) (Thread.memory th0))
-      (CLOSED: Memory.closed (Thread.memory th0))
-      (CONS: Local.promise_consistent th2.(Thread.local))
-  :
+      (CLOSED: Memory.closed (Thread.memory th0)):
     exists th1,
       (<<PROMISES: rtc (tau (@pred_step is_promise _)) th0 th1>>) /\
       (<<LOWER: rtc (tau lower_step) th1 th2>>) /\
       (<<MEM: th1.(Thread.memory) = th2.(Thread.memory)>>) /\
       (<<SC: th1.(Thread.sc) = th2.(Thread.sc)>>).
 Proof.
-  hexploit Thread.step_future; eauto. i. des.
   dup STEP. inv STEP.
   { exists th2. inv STEP1. ss. splits; eauto.
     econs; eauto. econs.
@@ -217,47 +357,118 @@ Proof.
     }
     { ss. }
   }
-  { inv STEP1. inv LOCAL0; ss.
-    { eapply step_split_pure; eauto; ss. }
-    { eapply step_split_pure; eauto; ss. }
-    { inv LOCAL1. ss. dup WRITE. inv WRITE. esplits.
-      { econs; [|econs]. eapply promise_step_tau_promise_step.
-        econs.
-        { econs; eauto. econs; ss. eapply TViewFacts.op_closed_released.
-          { eapply SC. }
-          { eauto. }
-          { eapply LOCAL. }
-          { eauto. }
-          { eapply Memory.write_op; eauto. }
-        }
-        { ss. }
-      }
-      { econs; [|econs]. eapply lower_step_tau_lower_step.
-        { econs.
-          { econs 2. econs; eauto; cycle 1.
-            { econs 3. econs; eauto; ss. econs; eauto.
-              eapply memory_lower_exists; eauto.
-              { eapply promise_memory_le; eauto. eapply LOCAL. }
-              { ss. }
-              { eapply Memory.remove_get0 in REMOVE. des. auto. }
-              { eapply Memory.promise_bot_none; eauto. eapply LOCAL. }
-            }
-            { ss. }
-          }
-          { ss. }
-          { ss. }
-          { ss. refl. }
-        }
-      }
-      { ss. }
-      { ss. }
-    }
-    { admit. }
-    { eapply step_split_pure; eauto; ss. }
-    { admit. }
-    { eapply step_split_pure; eauto; ss. }
+
+  inv STEP1. inv LOCAL0; ss.
+  { exploit step_split_pure; eauto; ss. i. des. esplits; eauto. }
+  { exploit step_split_pure; eauto; ss. i. des. esplits; eauto. }
+  { (* write *)
+    exploit split_write; try exact LOCAL1; eauto.
+    { destruct ord; ss. }
+    i. des.
+    esplits.
+    - econs 2; eauto. eapply promise_step_tau_promise_step. econs; eauto.
+    - econs 2; eauto. eapply lower_step_tau_lower_step.
+      econs; [econs; eauto|..]; eauto. refl.
+    - ss.
+    - inv WRITE. ss.
   }
-Admitted.
+  { (* update *)
+    exploit Local.read_step_future; eauto. i. des.
+    exploit split_write; try exact LOCAL2; eauto.
+    { destruct ordw; ss. }
+    i. des.
+    exploit reorder_read_promise_diff; try exact LOCAL1; eauto.
+    { inv WRITE. exploit MemoryFacts.write_time_lt; eauto. i.
+      ii. inv H. timetac.
+    }
+    i. des.
+    esplits.
+    - econs 2; eauto. eapply promise_step_tau_promise_step. econs; eauto.
+    - econs 2; eauto. eapply lower_step_tau_lower_step.
+      econs; [econs; eauto|..]; eauto. refl.
+    - ss.
+    - inv WRITE. ss.
+  }
+  { exploit step_split_pure; eauto; ss. i. des. esplits; eauto. }
+
+  { (* na write *)
+    clear STEP0. inv LOCAL1.
+    cut (exists th1 kinds' kind',
+            rtc (tau (@pred_step is_promise _)) (Thread.mk _ st1 lc1 sc1 mem1) th1 /\
+            Memory.write_na
+              (View.rlx (TView.cur (Local.tview lc1)) loc)
+              th1.(Thread.local).(Local.promises) th1.(Thread.memory)
+              loc from to val promises2 mem2 msgs kinds' kind' /\
+            th1.(Thread.state) = st1 /\
+            th1.(Thread.local).(Local.tview) = lc1.(Local.tview) /\
+            th1.(Thread.memory) = mem2 /\
+            th1.(Thread.sc) = sc1).
+    { i. des.
+      destruct th1. ss. subst. rewrite <- H2 in *.
+      esplits; eauto. econs 2; eauto. econs.
+      - econs.
+        + econs; cycle 1.
+          * econs 8. econs; eauto.
+          * ss.
+        + ss.
+        + refl.
+      - ss.
+    }
+
+    destruct lc1. ss.
+    remember (View.rlx (TView.cur tview) loc) as ts eqn:TS.
+    assert (LE: Time.le (View.rlx (TView.cur tview) loc) ts) by (subst; refl).
+    clear TS.
+    induction WRITE.
+    { inv WRITE. esplits.
+      - econs 2; eauto. eapply promise_step_tau_promise_step. econs; eauto.
+      - s. hexploit Memory.promise_get0; try exact PROMISE.
+        { inv PROMISE; ss. }
+        i. des.
+        hexploit Memory.get_ts; try exact GET_MEM. i. des.
+        { subst. inv WRITABLE. }
+        hexploit Memory.lower_exists_same; try exact GET_PROMISES; eauto. i.
+        hexploit Memory.lower_exists_same; try exact GET_MEM; eauto. i.
+        econs 1.
+        + ss.
+        + econs; eauto. econs 3; eauto; ss.
+          econs. apply Time.bot_spec.
+      - refl.
+      - refl.
+      - refl.
+      - refl.
+    }
+
+    exploit Memory.write_future; try exact WRITE_EX; try apply LOCAL; eauto.
+    { unguard. des; subst; ss. econs; ss. }
+    i. des.
+    exploit IHWRITE; eauto.
+    { eapply Memory.future_closed_timemap; eauto. }
+    { econs; try apply LOCAL; eauto.
+      eapply TView.future_closed; eauto. apply LOCAL. }
+    { econs. eapply TimeFacts.le_lt_lt; eauto. }
+    i. des.
+    exploit split_memory_write; try exact WRITE_EX.
+    { unguard. des; subst; ss. }
+    i. des.
+    exploit reorder_write_lower_rtc_promise; try exact x; try apply WRITE_LOWER; eauto.
+    { eapply Memory.promise_le; try eapply LOCAL; eauto. }
+    s. i. des.
+    esplits.
+    - econs 2; try exact STEPS. econs; [econs|].
+      + econs. econs. econs; eauto. econs; eauto.
+        unguard. des; subst; ss. econs. ss.
+      + ss.
+      + ss.
+    - econs 2; eauto.
+    - congr.
+    - congr.
+    - exploit memory_write_lower_refl_inv; try exact WRITE0. i. congr.
+    - congr.
+  }
+  { exploit step_split_pure; eauto; ss. i. des. esplits; eauto. }
+Qed.
+
 
 Definition delayed {lang} (st0 st1: lang.(Language.state))
            lc0 lc1 mem sc fin: Prop
@@ -288,12 +499,10 @@ Lemma delayed_future
       mem1 sc1
       lang (st0 st1: lang.(Language.state)) lc0 lc1 mem0 sc0 fin0 fin1
       (DELAYED: delayed st0 st1 lc0 lc1 mem0 sc0 fin0)
-
       (MEM: Memory.closed mem1)
       (SC: Memory.closed_timemap sc1 mem1)
       (LOCAL: Local.wf lc1 mem1)
       (FIN: fin1 <4= unchangable mem1 lc1.(Local.promises))
-
       (MEM_FUTURE: Memory.future mem0 mem1)
       (SC_FUTURE: TimeMap.le sc0 sc1)
       (FIN_FUTURE: fin0 <4= fin1)
